reflection: exposing the sort of pattern variables as sealed

ulib/experimental/FStar.InteractiveHelpers.Base.fst
@@ -567,12 +567,14 @@ and deep_apply_subst_in_pattern e pat subst =
                       ((pat, b) :: pats, subst)) patterns ([], subst)
     in
     Pat_Cons fv us patterns, subst
-  | Pat_Var bv ->
+  | Pat_Var bv st ->
+    let st = Sealed.seal (deep_apply_subst e (unseal st) subst) in
     let bv, subst = deep_apply_subst_in_bv e bv subst in
-    Pat_Var bv, subst
-  | Pat_Wild bv ->
+    Pat_Var bv st, subst
+  | Pat_Wild bv st ->
+    let st = Sealed.seal (deep_apply_subst e (unseal st) subst) in
     let bv, subst = deep_apply_subst_in_bv e bv subst in
-    Pat_Wild bv, subst
+    Pat_Wild bv st, subst
   | Pat_Dot_Term eopt ->
     Pat_Dot_Term (map_opt (fun t -> deep_apply_subst e t subst) eopt), subst
 
