tests/tactics/Synthesis.fst
@@ -56,9 +56,10 @@ let iszero (x : int) : int =
         let x = quote x in
         let t_int = quote int in
         let _f = fresh_bv () in
+        let tun = pack_ln Tv_Unknown in
         let t = Tv_Match x None
                     [(Pat_Constant (C_Int 0), pack (Tv_Const (C_Int 1)));
-                     (Pat_Wild _f, pack (Tv_Const (C_Int 0)))] in
+                     (Pat_Wild _f (seal tun), pack (Tv_Const (C_Int 0)))] in
         exact (pack t))
 
 let _ = assert (iszero 0 = 1)
